# Exercise 1

1) Answer B: ``ğœ†ğ‘¥ğ‘¦.ğ‘¥ğ‘§ == ğœ†ğ‘šğ‘›.ğ‘šğ‘§``

2) Answer C: ``ğœ†ğ‘¥ğ‘¦.ğ‘¥ğ‘¥ğ‘¦ == ğœ†ğ‘.(ğœ†ğ‘.ğ‘ğ‘ğ‘)``

3) Answer B: ``ğœ†ğ‘¥ğ‘¦ğ‘§.ğ‘§ğ‘¥ == ğœ†ğ‘¡ğ‘œğ‘ .ğ‘ ğ‘¡``

# Excercise 2:

**Combinators:**

1. Yes
2. No, `ğ‘§` is a free variable
3. Yes
4. Yes
5. No, `ğ‘§` is a free variable

**Normal form or Divergence?**

1. Normal form: 

2. Divergent, because `(ğœ†ğ‘§.ğ‘§ğ‘§)(ğœ†ğ‘¦.ğ‘¦ğ‘¦)` is alpha equivalent to `(ğœ†ğ‘¥.ğ‘¥ğ‘¥)(ğœ†ğ‘¥.ğ‘¥ğ‘¥)` (the omega term)

3. Normal form
```
(ğœ†ğ‘¥.ğ‘¥ğ‘¥ğ‘¥)ğ‘§
ğ‘§ğ‘§ğ‘§
```

**Beta reduce:**

1.

```
(ğœ†ğ‘ğ‘ğ‘.ğ‘ğ‘ğ‘)ğ‘§ğ‘§(ğœ†ğ‘¤ğ‘£.ğ‘¤)
(ğœ†ğ‘(ğœ†ğ‘(ğœ†ğ‘.ğ‘ğ‘ğ‘))ğ‘§ğ‘§(ğœ†ğ‘¤ğ‘£.ğ‘¤)
[ğ‘ âˆ¶= ğ‘§]
(ğœ†ğ‘(ğœ†ğ‘.ğ‘ğ‘ğ‘§))ğ‘§(ğœ†ğ‘¤ğ‘£.ğ‘¤)
[ğ‘ âˆ¶= ğ‘§]
(ğœ†ğ‘.ğ‘ğ‘§ğ‘§)(ğœ†ğ‘¤ğ‘£.ğ‘¤)
[ğ‘ âˆ¶= ğœ†ğ‘¤ğ‘£.ğ‘¤]
(ğœ†ğ‘¤ğ‘£.ğ‘¤)ğ‘§ğ‘§
(ğœ†ğ‘¤(ğœ†ğ‘£.ğ‘¤))ğ‘§ğ‘§
[ğ‘¤ âˆ¶= ğ‘§]
(ğœ†ğ‘£.ğ‘§)ğ‘§
[v âˆ¶= ğ‘§]
ğ‘§
```

2. 
```
(ğœ†ğ‘¥.ğœ†ğ‘¦.ğ‘¥ğ‘¦ğ‘¦)(ğœ†ğ‘.ğ‘)ğ‘
(ğœ†ğ‘¥(ğœ†ğ‘¦.ğ‘¥ğ‘¦ğ‘¦))(ğœ†ğ‘.ğ‘)ğ‘
[ğ‘¥ âˆ¶= ğœ†ğ‘.ğ‘]
(ğœ†ğ‘¦(ğœ†ğ‘.ğ‘)ğ‘¦ğ‘¦)ğ‘
[ğ‘¦ âˆ¶= ğ‘]
(ğœ†ğ‘.ğ‘)ğ‘ğ‘
[ğ‘ âˆ¶= ğ‘]
ğ‘ğ‘
```

3. 
```
(ğœ†ğ‘¦.ğ‘¦)(ğœ†ğ‘¥.ğ‘¥ğ‘¥)(ğœ†ğ‘§.ğ‘§ğ‘)
[ğ‘¦ âˆ¶= ğœ†ğ‘¥.ğ‘¥ğ‘¥]
(ğœ†ğ‘¥.ğ‘¥ğ‘¥)(ğœ†ğ‘§.ğ‘§ğ‘)
[ğ‘¥ âˆ¶= ğœ†ğ‘§.ğ‘§ğ‘]
(ğœ†ğ‘§.ğ‘§ğ‘)(ğœ†ğ‘§.ğ‘§ğ‘)
[z âˆ¶= ğœ†ğ‘§.ğ‘§ğ‘]
(ğœ†ğ‘§.ğ‘§ğ‘)ğ‘
[z âˆ¶= ğ‘]
ğ‘ğ‘
```

4. 
```
(ğœ†ğ‘§.ğ‘§)(ğœ†ğ‘§.ğ‘§ğ‘§)(ğœ†ğ‘§.ğ‘§ğ‘¦)
(ğœ†ğ‘§.ğ‘§ğ‘§)(ğœ†ğ‘§.ğ‘§ğ‘¦)
[z âˆ¶= ğœ†ğ‘§.ğ‘§ğ‘¦]
(ğœ†ğ‘§.ğ‘§ğ‘¦)(ğœ†ğ‘§.ğ‘§ğ‘¦)
[z âˆ¶= ğœ†ğ‘§.ğ‘§ğ‘¦]
(ğœ†ğ‘§.ğ‘§ğ‘¦)ğ‘¦
ğ‘¦ğ‘¦
```

5.
```
(ğœ†ğ‘¥.ğœ†ğ‘¦.ğ‘¥ğ‘¦ğ‘¦)(ğœ†ğ‘¦.ğ‘¦)ğ‘¦
(ğœ†ğ‘¥(ğœ†ğ‘¦.ğ‘¥ğ‘¦ğ‘¦))(ğœ†ğ‘¦.ğ‘¦)ğ‘¦
[ğ‘¥ âˆ¶= ğœ†ğ‘¦.ğ‘¦]
(ğœ†ğ‘¦.(ğœ†ğ‘¦.ğ‘¦)ğ‘¦ğ‘¦)ğ‘¦
ğ‘¦ğ‘¦
```

6.
```
(ğœ†ğ‘.ğ‘ğ‘)(ğœ†ğ‘.ğ‘ğ‘)ğ‘
[ğ‘ âˆ¶= ğœ†ğ‘.ğ‘ğ‘]
(ğœ†ğ‘.ğ‘ğ‘)(ğœ†ğ‘.ğ‘ğ‘)ğ‘
[ğ‘ âˆ¶= ğœ†ğ‘.ğ‘ğ‘]
(ğœ†ğ‘.ğ‘ğ‘)(ğ‘)ğ‘
[ğ‘ âˆ¶= ğ‘]
ğ‘ğ‘ğ‘
```
7.
```
(ğœ†ğ‘¥ğ‘¦ğ‘§.ğ‘¥ğ‘§(ğ‘¦ğ‘§))(ğœ†ğ‘¥.ğ‘§)(ğœ†ğ‘¥.ğ‘)
(ğœ†ğ‘¥(ğœ†ğ‘¦ğ‘§.ğ‘¥ğ‘§(ğ‘¦ğ‘§)))(ğœ†ğ‘¥.ğ‘§)(ğœ†ğ‘¥.ğ‘)
(ğœ†ğ‘¥(ğœ†ğ‘¦(ğœ†ğ‘§.ğ‘¥ğ‘§(ğ‘¦ğ‘§))))(ğœ†ğ‘¥.ğ‘§)(ğœ†ğ‘¥.ğ‘)
[ğ‘¥ âˆ¶= (ğœ†ğ‘¥.ğ‘§)]
(ğœ†ğ‘¦.ğœ†ğ‘§1(ğœ†ğ‘¥.ğ‘§)ğ‘§1(ğ‘¦ğ‘§1))(ğœ†ğ‘¥.ğ‘)        \\ Rename leftmost z to z1
[ğ‘¦ âˆ¶= (ğœ†ğ‘¥.ğ‘)]
(ğœ†ğ‘§1(ğœ†ğ‘¥.ğ‘§)(ğ‘§1)((ğœ†ğ‘¥.ğ‘)ğ‘§1))
(ğœ†ğ‘§1.ğ‘§((ğœ†ğ‘¥.ğ‘)(ğ‘§1)))              \\ Our leftmost, outermost lambda has no remaining arguments to be applied so we now examine the terms nested within to see if they are in normal form. 
[ğ‘§1 âˆ¶= (ğœ†ğ‘¥.ğ‘§)]
(ğœ†ğ‘§1.ğ‘§((ğœ†ğ‘¥.ğ‘)(ğ‘§1)))
(ğœ†ğ‘§1.ğ‘§ğ‘)
```